Add comments

proof_of_soundness/EvalRules.v
@@ -1,274 +1,291 @@
+(*  EvalRules.v
+    Definition of the big-step operational semantics for the language
+    as a relation, definition of macro substitution as relations, and lemmas
+    concerning these relations.
+*)
+
 Require Import
-  Coq.Lists.List
+Coq.Lists.List
   Coq.Logic.Classical_Prop
   Coq.Strings.String
   Coq.ZArith.ZArith.
 
 From Cpp2C Require Import
   ConfigVars
-  MapTheorems
+  MapLemmas
   Syntax.
 
-(* Macro substitution.
-   Check this for details on nested calls to macros:
-   https://gcc.gnu.org/onlinedocs/cpp/Argument-Prescan.html
-   Currently we don't supported macro calls in macro arguments.
- *)
-Fixpoint msub
-  (p : string) (e : expr) (mexpr : expr) : expr :=
-  match mexpr with
-  | Num z => Num z
-  | Var x =>
-    match (p =? x)%string with
-    | true => e
-    | false => Var x
-    end
-  | ParenExpr e0 => ParenExpr (msub p e e0)
-  | UnExpr uo e0 => UnExpr uo (msub p e e0)
-  | BinExpr bo e1 e2 => BinExpr bo (msub p e e1) (msub p e e2)
-    (* TODO: Fix these two once we add pointers *)
-  | Assign x e0 => match (p =? x)%string with
-    (* Right now we only substitute the LHS of assignments if
-       the expression to plug in is also simply a variable *)
-    | true => match e with
-      | (Var y) => Assign y (msub p e e0)
-      | _ => Assign x (msub p e e0)
-      end
-    | _ => Assign x (msub p e e0)
-    end
-  (* FIXME: This doesn't match the actual semantics of macro expansion
-            See the Google Doc *)
-  | CallOrInvocation x es => CallOrInvocation x es
-end.
-
-
+(*  Macro substitution, one parameter at a time.
+    Check this for details on nested calls to macros:
+    https://gcc.gnu.org/onlinedocs/cpp/Argument-Prescan.html
+    Currently we don't support macro calls in macro arguments.
+*)
 Inductive MSub : string -> expr -> expr -> expr -> Prop :=
   | MS_Num : forall p e z,
+    (*  Numerals never get substituted *)
     MSub p e (Num z) (Num z)
   | MS_Var_Replace : forall p e x,
+    (*  Variables only get substituted if the var's id
+        matches that of the parameter we are currently trying
+        to substitute into the expression *)
     p = x ->
     MSub p e (Var x) e
   | MS_Var_No_Replace : forall p e x,
+    (*  If a variable's id doesn't match the parameter we are searching for,
+        then no substitution is performed *)
     p <> x ->
     MSub p e (Var x) (Var x)
   | MS_PareExpr : forall p e e0 e0',
+    (*  Substitute the inner expression and return the result *)
     MSub p e e0 e0' ->
     MSub p e (ParenExpr e0) (ParenExpr e0')
   | MS_UnExpr : forall p e uo e0 e0',
+    (*  Substitute the inner expression and return the result *)
     MSub p e e0 e0' ->
     MSub p e (UnExpr uo e0) (UnExpr uo e0')
   | MS_BinExpr : forall p e bo e1 e2 e1' e2',
+    (*  Substitute the left operand *)
     MSub p e e1 e1' ->
+    (*  Substitute the right operand *)
     MSub p e e2 e2' ->
+    (*  Return the result *)
     MSub p e (BinExpr bo e1 e2) (BinExpr bo e1' e2')
   | MS_Assign_Replace : forall p e x y e0 e0',
+    (*  Since we don't have a separate evaluation defined
+        for L-values, we only substitute the variable on the
+        left-hand-side of an assignment if two criteria are met:
+        1)  The variable's id matches that of the parameter we are
+            searching for
+        2)  The expression to substitute into the main expression
+            is also a variable *)
     p = x ->
     e = Var y ->
     MSub p e e0 e0' ->
     MSub p e (Assign x e0) (Assign y e0')
   | MS_Assign_No_Replace : forall p e x e0 e0',
+    (*  If either of the above criteria are not met, then
+        we do not perform a substitution *)
     p <> x ->
     MSub p e e0 e0' ->
     MSub p e (Assign x e0) (Assign x e0')
   | MS_Call_Or_Invocation : forall p e x es es',
+    (*  We currently do not substitute calls or invocations, but
+        we do recursively perform substitutions in all their arguments *)
     MSubList p e es es' ->
     MSub p e (CallOrInvocation x es) (CallOrInvocation x es')
 with MSubList : string -> expr -> list expr -> list expr -> Prop :=
   | MSL_nil : forall p e,
+    (*  End of the list - no more substitutions *)
     MSubList p e nil nil
   | MSL_cons : forall p e e0 e0' es0 es0',
+    (*  Subsitutute the head of the list *)
     MSub p e e0 e0' ->
+    (*  Substitute the rest of the list *)
     MSubList p e es0 es0' ->
+    (*  The result is the transformed head of the list prepended to the
+        transformed tail of the list *)
     MSubList p e (e0::es0) (e0'::es0').
 
+(*  Macro substitution for a list of parameters, and expressions to
+    replace them with *)
+Inductive MacroSubst :
+  list string -> list expr -> expr -> expr -> Prop :=
+  | MacroSubst_nil : forall mexpr,
+    (*  No more substitutions necessary *)
+    MacroSubst nil nil mexpr mexpr
+  | MacroSubst_cons : forall p e ps es mexpr ef ef',
+    (*  Substitute the first argument *)
+    MSub p e mexpr ef ->
+    (*  Substitute the remaining arguments *)
+    MacroSubst ps es ef ef' ->
+    (*  Return the fully-substituted expression *)
+    MacroSubst (p::ps) (e::es) mexpr ef'.
 
-(* Right now, a term that fails to evaluate will simply get "stuck";
-   i.e. it will fail to be reduced further. *)
+(*  Right now, a term that fails to evaluate will simply get "stuck";
+    i.e. it will fail to be reduced further. *)
 Inductive EvalExpr:
   store -> environment -> environment ->
   function_table -> macro_table ->
   expr ->
   Z -> store -> Prop :=
-  (* Numerals evaluate to their integer representation and do not
-     change the store *)
+  (*  Numerals evaluate to their integer representation and do not
+      change the store *)
   | E_Num : forall S E G F M z S',
     NatMap.Equal S S' ->
     EvalExpr S E G F M (Num z) z S'
-  (* Local variable lookup *)
+  (*  Local variable lookup *)
   | E_LocalVar : forall S E G F M x l v S',
-    (* Store does not change *)
+    (*  Store does not change *)
     NatMap.Equal S S' ->
-    (* Variable is found in local environment *)
+    (*  Variable is found in local environment *)
     StringMap.MapsTo x l E ->
-    (* L-value maps to an R-value *)
+    (*  L-value maps to an R-value *)
     NatMap.MapsTo l v S ->
     EvalExpr S E G F M (Var x) v S'
-  (* Global variable lookup *)
+  (*  Global variable lookup *)
   | E_GlobalVar : forall S E G F M x l v S',
-    (* Store does not change *)
+    (*  Store does not change *)
     NatMap.Equal S S' ->
-  (* Local variables shadow global variables, so only if a local
-     variable lookup fails do we check the global environment. *)
+  (*  Local variables shadow global variables, so only if a local
+      variable lookup fails do we check the global environment. *)
     ~ StringMap.In x E->
-    (* Variable is found in global environment *)
+    (*  Variable is found in global environment *)
     StringMap.MapsTo x l G ->
-    (* L-value maps to R-value *)
+    (*  L-value maps to R-value *)
     NatMap.MapsTo l v S ->
     EvalExpr S E G F M (Var x) v S'
-  (* Parenthesized expressions evaluate to themselves. *)
+  (*  Parenthesized expressions evaluate to themselves. *)
   | E_ParenExpr : forall S E G F M e0 v S',
-    (* Evaluate the inner expression *)
+    (*  Evaluate the inner expression *)
     EvalExpr S E G F M e0 v S' ->
     EvalExpr S E G F M (ParenExpr e0) v S'
-  (* Unary expressions *)
+  (*  Unary expressions *)
   | E_UnExpr : forall S E G F M S' uo e0 v,
-    (* Evaluate the inner expression *)
+    (*  Evaluate the inner expression *)
     EvalExpr S E G F M e0 v S' ->
-    (* Perform the unary operations on the value obtained *)
+    (*  Perform the unary operations on the value obtained *)
     EvalExpr S E G F M (UnExpr uo e0) ((unop_to_op uo) v) S'
-  (* Binary expressions. Left operands are evaluated first. *)
-  (* NOTE: Evaluation rules do not handle operator precedence.
-     The parser must use a concrete syntax to generate a parse tree
-     with the appropriate precedence levels in it. *)
+  (*  Binary expressions. Left operands are evaluated first. *)
+  (*  NOTE: Evaluation rules do not handle operator precedence.
+      The parser must use a concrete syntax to generate a parse tree
+      with the appropriate precedence levels in it. *)
   | E_BinExpr : forall S E G F M bo e1 e2 v1 v2 S' S'',
-    (* Evaluate the left operand *)
+    (*  Evaluate the left operand *)
     EvalExpr S E G F M e1 v1 S' ->
-    (* Evaluate the right operand *)
+    (*  Evaluate the right operand *)
     EvalExpr S' E G F M e2 v2 S'' ->
-    (* Perform the binary operation on the values obtained *)
+    (*  Perform the binary operation on the values obtained *)
     EvalExpr S E G F M (BinExpr bo e1 e2) ((binop_to_op bo) v1 v2) S''
-  (* Variable assignments update the store by adding a new L-value to
-     R-value mapping or by overriding an existing one.
-     The R-value is returned along with the updated state. *)
-  (* Local variable assignment overrides global variable assignment. *)
+  (*  Variable assignments update the store by adding a new L-value to
+      R-value mapping or by overriding an existing one.
+      The R-value is returned along with the updated state. *)
+  (*  Local variable assignment overrides global variable assignment. *)
   | E_Assign_Local : forall S E G F M l x e0 v S' S'',
+    (*  Find the variable in the local environment *)
     StringMap.MapsTo x l E ->
+    (*  Evaluate the RHS of the assignment *)
     EvalExpr S E G F M e0 v S' ->
+    (*  Add the new mapping to the store *)
     NatMap.Equal S'' (NatMapProperties.update S (NatMap.add l v (NatMap.empty Z))) ->
     EvalExpr S E G F M (Assign x e0) v S''
-  (* Global variable assignment *)
+  (*  Global variable assignment *)
   | E_Assign_Global : forall S E G F M l x e0 v S' S'',
+    (*  The variable is not found in the local environment *)
     ~ StringMap.In x E ->
+    (*  Find the variable in the global environment *)
     StringMap.MapsTo x l G ->
+    (*  Evaluate the RHS of the assignment *)
     EvalExpr S E G F M e0 v S' ->
+    (*  Add the new mapping to the store *)
     NatMap.Equal S'' (NatMapProperties.update S (NatMap.add l v (NatMap.empty Z))) ->
     EvalExpr S E G F M (Assign x e0) v S''
-  (* For function calls, we perform the following steps:
-     1) Evaluate arguments
-     2) Map parameters to arguments in function local environment,
-        which is based on the global environment
-     3) Evaluate the function's statement
-     4) Evaluate the function's return expression
-     4.5) Remove the mappings that were added to the store for the function
-          call
-     5) Return the return value and store *)
+  (*  For function calls, we perform the following steps:
+      1) Evaluate arguments
+      2) Map parameters to arguments in function local environment,
+         which is based on the global environment
+      3) Evaluate the function's statement
+      4) Evaluate the function's return expression
+      4.5) Remove the mappings that were added to the store for the function
+           call
+      5) Return the return value and store *)
   | E_FunctionCall:
     forall S E G F M x es params fstmt fexpr l ls
            Ef Sargs S' S'' S''' S'''' S''''' v vs,
-    (* TODO: Things to consider :
-       - Should all functions have unique names?
+    (*  TODO: Things to consider :
+        - Should all functions have unique names?
+        - Some of these premises could probably be removed
     *)
-    (* Macro definitions shadow function definitions, so function calls
-       only occur if a macro definition is not found *)
+    (*  Macro definitions shadow function definitions, so function calls
+        only occur if a macro definition is not found *)
     ~ StringMap.In x M ->
-    (* Function name maps to some function *)
+    (*  Function name maps to some function *)
     StringMap.MapsTo x (params, fstmt, fexpr) F ->
-    (* Parameters should all be unique *)
+    (*  Parameters should all be unique *)
     NoDup params ->
-    (* Evaluate the function's arguments *)
+    (*  Evaluate the function's arguments *)
     EvalExprList S E G F M params es vs S' Ef Sargs l ls ->
-    (* Create the function environment *)
+    (*  Create the function environment *)
     StringMap.Equal Ef (StringMapProperties.of_list (combine params ls)) ->
-    (* Create a store for mapping L-values to the arguments to in the store.
+    (*  Create a store for mapping L-values to the arguments to in the store.
        Possibly provable but easier to just assert here *)
     NatMap.Equal Sargs (NatMapProperties.of_list (combine ls vs)) ->
-    (* All the L-values used in the argument store do not appear in the original store.
+    (*  All the L-values used in the argument store do not appear in the original store.
        We could possibly prove this, but it is easier to put it here. *)
     NatMapProperties.Disjoint S' Sargs ->
-    (* Combine the argument store into the original store *)
+    (*  Combine the argument store into the original store *)
     NatMap.Equal S'' (NatMapProperties.update S' Sargs) ->
-    (* Evaluate the function's body *)
+    (*  Evaluate the function's body *)
     EvalStmt S'' Ef G F M fstmt S''' ->
     EvalExpr S''' Ef G F M fexpr v S'''' ->
-    (* Only keep in the store the L-value mappings that were there when
-       the function was called; i.e., remove from the store all mappings
-       whose L-value is in Ef/Sargs. *)
+    (*  Only keep in the store the L-value mappings that were there when
+        the function was called; i.e., remove from the store all mappings
+        whose L-value is in Ef/Sargs. *)
     NatMap.Equal S''''' (NatMapProperties.restrict S'''' S) ->
     EvalExpr S E G F M (CallOrInvocation x es) v S'''''
-  (* Macro invocation *)
+  (*  Macro invocation *)
   | E_MacroInvocation :
     forall S E G F M x params es mexpr M' ef S' v,
-    (* TODO: Things to consider:
+    (*  TODO: Things to consider:
      - How to handle nested macros?
      *)
-    (* Macro definitions shadow function definitions, so if a macro
-       definition is found, we don't even check the function list.
-       However, when we execute the macro's body, we need to remove
-       the current macro definition from the list of macro definitions
-       to avoid nested macros from being expanded. *)
+    (*  Macro definitions shadow function definitions, so if a macro
+        definition is found, we don't even check the function list.
+        However, when we execute the macro's body, we need to remove
+        the current macro definition from the list of macro definitions
+        to avoid nested macros from being expanded. *)
     StringMap.MapsTo x (params, mexpr) M ->
-    (* Remove the macro from the macro table to avoid recursively
-       expanding macros. We could express this using StringMap.Equal,
-       but it is easier for the proof if we Logic.eq instead. *)
+    (*  Remove the macro from the macro table to avoid recursively
+        expanding macros. We could express this using StringMap.Equal,
+        but it is easier for the proof if we Logic.eq instead. *)
     M' = (StringMap.remove x M) ->
-    (* No duplicate parameters *)
+    (*  No duplicate parameters *)
     NoDup params ->
-    (* Perform the macro substitution *)
+    (*  Perform the macro substitution *)
     MacroSubst params es mexpr ef ->
-    (* Evalue the fully-substituted macro body
-       under the caller's environment *)
+    (*  Evalue the fully-substituted macro body
+        under the caller's environment *)
     EvalExpr S E G F M' ef v S' ->
     EvalExpr S E G F M (CallOrInvocation x es) v S'
 with EvalExprList :
   store -> environment -> environment -> function_table -> macro_table ->
   list string -> list expr -> list Z -> store -> environment -> store ->
   nat -> list nat -> Prop :=
-  (* End of arguments *)
+  (*  End of arguments *)
   | E_ExprList_nil : forall Sprev Ecaller G F M Snext,
     NatMap.Equal Sprev Snext ->
     EvalExprList Sprev Ecaller G F M nil nil nil Snext (StringMap.empty nat) (NatMap.empty Z)
       1 (0 :: nil)
-  (* There are arguments left to evaluate *)
+  (*  There are arguments left to evaluate *)
   | E_ExprList_cons : forall Sprev Ecaller G F M p e v Snext ps es vs Sfinal Ef' Sargs' l ls,
-    (* Evaluate the first expression using the caller's environment *)
+    (*  Evaluate the first expression using the caller's environment *)
     EvalExpr Sprev Ecaller G F M e v Snext ->
-    (* Evaluate the remaining expressions *)
+    (*  Evaluate the remaining expressions *)
     EvalExprList Snext Ecaller G F M ps es vs Sfinal Ef' Sargs' l ls ->
-    (* The L-value to add is not in the store *)
+    (*  The L-value to add is not in the store *)
     ~ NatMap.In l Sargs' ->
-    (* The parameter to add is not in the environment *)
+    (*  The parameter to add is not in the environment *)
     NoDup (p::ps) ->
     ~ StringMap.In p Ef' ->
-    (* Return the final environment *)
+    (*  Return the final environment *)
     EvalExprList  Sprev Ecaller G F M (p::ps) (e::es) (v::vs) Sfinal
                   (StringMap.add p l Ef') (NatMap.add l v Sargs') l ( l :: ls)
-with MacroSubst :
-  list string -> list expr -> expr -> expr -> Prop :=
-  | MacroSubst_nil : forall mexpr,
-    (* No more substitutions necessary *)
-    MacroSubst nil nil mexpr mexpr
-  | MacroSubst_cons : forall p e ps es mexpr ef ef',
-    (* Substitute the first argument *)
-    MSub p e mexpr ef ->
-    (* Substitute the remaining arguments *)
-    MacroSubst ps es ef ef' ->
-    (* Return the fully-substituted expression *)
-    MacroSubst (p::ps) (e::es) mexpr ef'
 with EvalStmt :
   store -> environment -> environment ->
   function_table -> macro_table ->
   stmt ->
   store -> Prop :=
-  (* A skip statement does not change the state *)
+  (*  A skip statement does not change the state *)
   | E_Skip : forall S E G F M S',
     NatMap.Equal S S' ->
     EvalStmt S E G F M Skip S'.
 
 
+(*  Custom induction scheme for Macro substitution *)
 Scheme MSub_mut := Induction for MSub Sort Prop
 with MSubList_mut := Induction for MSubList Sort Prop.
 
-
+(*  Given the same inputs, single argument macro substitution will
+    always return the same result *)
 Lemma MSub_deterministic : forall p e mexpr ef,
   MSub p e mexpr ef ->
   forall ef0,
@@ -307,6 +324,8 @@ Proof.
 Qed.
 
 
+(*  Given the same inputs, multiple argument macro substitution will
+    always return the same result *)
 Lemma MacroSubst_deterministic : forall params es mexpr ef,
   MacroSubst params es mexpr ef ->
   forall ef0,
@@ -322,6 +341,9 @@ Proof.
 Qed.
 
 
+(*  If the body of a macro substitution is a numeral, then after single
+    argument substitution, the fully-substituted expression will be the
+    same numeral *)
 Lemma MSub_mexpr_Num_ef_Num : forall p e z ef,
   MSub p e (Num z) ef ->
   ef = Num z.
@@ -331,29 +353,35 @@ Proof.
 Qed.
 
 
+(*  If the body of a macro substitution is a numeral, then after multiple
+    argument substitution, the fully-substituted expression will be the
+    same numeral *)
 Lemma MacroSubst_mexpr_Num_ef_Num : forall params es z ef,
   MacroSubst params es (Num z) ef ->
   ef = Num z.
 Proof.
   intros. remember (Num z). induction H.
-  - (* MacroSubst nil *)
+  - (*  MacroSubst nil *)
     auto.
-  - (* MacroSubst cons *)
+  - (*  MacroSubst cons *)
     subst. apply MSub_mexpr_Num_ef_Num in H. subst.
     auto.
 Qed.
 
 
-(* The following lemmas involve all parts of program evaluation
-   (e.g., expression, argument list, and statement evaluation).
-   Coq's built-in induction tactic is not powerful enough to provide
-   us with the induction hypotheses necessary to prove these lemmas, so
-   we must define our own induction schema for these proofs *)
+(*  The following lemmas involve all parts of program evaluation
+    (e.g., expression, argument list, and statement evaluation).
+    Coq's built-in induction tactic is not powerful enough to provide
+    us with the induction hypotheses necessary to prove these lemmas, so
+    we must define our own induction schema for these proofs *)
 Scheme EvalExpr_mut := Induction for EvalExpr Sort Prop
 with EvalStmt_mut := Induction for EvalStmt Sort Prop
 with EvalExprList_mut := Induction for EvalExprList Sort Prop.
 
 
+(*  If a statement terminates under some context, then it will also
+    terminate under a context in which a new function name has been
+    added to the function table *)
 Lemma EvalStmt_notin_F_add_EvalStmt : forall S E G F M stmt S',
   EvalStmt S E G F M stmt S' ->
   forall x fdef,
@@ -366,9 +394,9 @@ Proof.
   Instead I have opted to use our custom schema here so that it may serve
   as a simple demonstration of how to use schemas *)
   intros. apply (
-    (* First we apply the appropriate schema like a tactic *)
+    (*  First we apply the appropriate schema like a tactic *)
     EvalStmt_mut
-      (* Then we have to define a custom inductive hypothesis for each Prop
+      (*  Then we have to define a custom inductive hypothesis for each Prop
          that the one we are inducting over is mutually inductive with
          (in this case just the EvalStmt Prop since statement evaluation
          currently only includes skip statements, which don't
@@ -379,6 +407,9 @@ Proof.
 Qed.
 
 
+(*  If a statement terminates under some context, then it will also
+    terminate under a context in which a set of new function names have been
+    added to the function table *)
 Lemma EvalStmt_Disjoint_update_F_EvalStmt : forall S E G F M stmt S',
   EvalStmt S E G F M stmt S' ->
   forall F',
@@ -389,6 +420,9 @@ Proof.
 Qed.
 
 
+(*  If an expression terminates under some context, then it will also
+    terminate under a context in which a new function name has been
+    added to the function table *)
 Lemma EvalExpr_notin_F_add_EvalExpr : forall S E G F M e v S',
   EvalExpr S E G F M e v S' ->
   forall x fdef,
@@ -397,17 +431,17 @@ Lemma EvalExpr_notin_F_add_EvalExpr : forall S E G F M e v S',
 Proof.
   apply (
     EvalExpr_mut
-      (* EvalExpr *)
+      (*  EvalExpr *)
       (fun S E G F M e v S' (h : EvalExpr S E G F M e v S' ) =>
         forall x fdef,
         ~ StringMap.In x F ->
         EvalExpr S E G (StringMap.add x fdef F) M e v S' )
-      (* EvalStmt *)
+      (*  EvalStmt *)
       (fun S E G F M stmt S' (h : EvalStmt S E G F M stmt S' ) =>
         forall x fdef,
         ~ StringMap.In x F ->
         EvalStmt S E G (StringMap.add x fdef F) M stmt S' )
-      (* EvalExprList *)
+      (*  EvalExprList *)
       (fun Sprev Ecaller G F M ps es vs Snext Ef Sargs l ls (h : EvalExprList Sprev Ecaller G F M ps es vs Snext Ef Sargs l ls) =>
         forall x fdef,
         ~ StringMap.In x F ->
@@ -429,6 +463,9 @@ Proof.
 Qed.
 
 
+(*  If an expression terminates under some context, then it will also
+    terminate under a context in which a set of new function names have been
+    added to the function table *)
 Lemma EvalExpr_Disjoint_update_F_EvalExpr : forall S E G F M e v S',
   EvalExpr S E G F M e v S' ->
   forall F',
@@ -437,17 +474,17 @@ Lemma EvalExpr_Disjoint_update_F_EvalExpr : forall S E G F M e v S',
 Proof.
   apply (
     EvalExpr_mut
-      (* EvalExpr *)
+      (*  EvalExpr *)
       (fun S E G F M e v S' (h : EvalExpr S E G F M e v S' ) =>
         forall F',
           StringMapProperties.Disjoint F F' ->
           EvalExpr S E G (StringMapProperties.update F F') M e v S' )
-      (* EvalStmt *)
+      (*  EvalStmt *)
       (fun S E G F M stmt S' (h : EvalStmt S E G F M stmt S' ) =>
         forall F',
           StringMapProperties.Disjoint F F' ->
           EvalStmt S E G (StringMapProperties.update F F') M stmt S' )
-      (* EvalExprList *)
+      (*  EvalExprList *)
       (fun Sprev Ecaller G F M ps es vs Snext Ef Sargs l ls (h : EvalExprList Sprev Ecaller G F M ps es vs Snext Ef Sargs l ls) =>
         forall F',
           StringMapProperties.Disjoint F F' ->
@@ -475,6 +512,10 @@ Proof.
 Qed.
 
 
+(*  If an expression terminates under some context, then it will also
+    terminate under a context in which a set of function names that weren't
+    in the original function table to begin with have been removed from
+    the function table *)
 Lemma EvalExpr_Disjoint_diff_F_EvalExpr : forall S E G F M e v S',
   EvalExpr S E G F M e v S' ->
   forall F',
@@ -483,17 +524,17 @@ Lemma EvalExpr_Disjoint_diff_F_EvalExpr : forall S E G F M e v S',
 Proof.
   apply (
     EvalExpr_mut
-      (* EvalExpr *)
+      (*  EvalExpr *)
       (fun S E G F M e v S' (h : EvalExpr S E G F M e v S' ) =>
         forall F',
           StringMapProperties.Disjoint F F' ->
           EvalExpr S E G (StringMapProperties.diff F F') M e v S' )
-      (* EvalStmt *)
+      (*  EvalStmt *)
       (fun S E G F M stmt S' (h : EvalStmt S E G F M stmt S' ) =>
         forall F',
           StringMapProperties.Disjoint F F' ->
           EvalStmt S E G (StringMapProperties.diff F F') M stmt S' )
-      (* EvalExprList *)
+      (*  EvalExprList *)
       (fun Sprev Ecaller G F M ps es vs Snext Ef Sargs l ls (h : EvalExprList Sprev Ecaller G F M ps es vs Snext Ef Sargs l ls) =>
         forall F',
           StringMapProperties.Disjoint F F' ->
@@ -521,6 +562,9 @@ Proof.
 Qed.
 
 
+(*  If an expression list terminates under some context, then it will also
+    terminate under a context in which a new function name has been
+    added to the function table *)
 Lemma EvalExprList_notin_F_add_EvalExprList : forall S E G F M ps es vs S' Ef Sargs l ls,
   EvalExprList S E G F M ps es vs S' Ef Sargs l ls ->
   forall x fdef,
@@ -529,17 +573,17 @@ Lemma EvalExprList_notin_F_add_EvalExprList : forall S E G F M ps es vs S' Ef Sa
 Proof.
   apply (
     EvalExprList_mut
-      (* EvalExpr *)
+      (*  EvalExpr *)
       (fun S E G F M e v S' (h : EvalExpr S E G F M e v S' ) =>
         forall x fdef,
         ~ StringMap.In x F ->
         EvalExpr S E G (StringMap.add x fdef F) M e v S' )
-      (* EvalStmt *)
+      (*  EvalStmt *)
       (fun S E G F M stmt S' (h : EvalStmt S E G F M stmt S' ) =>
         forall x fdef,
         ~ StringMap.In x F ->
         EvalStmt S E G (StringMap.add x fdef F) M stmt S' )
-      (* EvalExprList *)
+      (*  EvalExprList *)
       (fun Sprev Ecaller G F M ps es vs Snext Ef Sargs l ls (h : EvalExprList Sprev Ecaller G F M ps es vs Snext Ef Sargs l ls) =>
         forall x fdef,
         ~ StringMap.In x F ->
@@ -560,6 +604,9 @@ Proof.
 Qed.
 
 
+(*  If an expression list terminates under some context, then it will also
+    terminate under a context in which a set of new function names have been
+    added to the function table *)
 Lemma EvalExprList_Disjoint_update_F_EvalExprList : forall S E G F M ps es vs S' Ef Sargs l ls,
   EvalExprList S E G F M ps es vs S' Ef Sargs l ls ->
   forall F',
@@ -568,17 +615,17 @@ Lemma EvalExprList_Disjoint_update_F_EvalExprList : forall S E G F M ps es vs S'
 Proof.
   apply (
     EvalExprList_mut
-      (* EvalExpr *)
+      (*  EvalExpr *)
       (fun S E G F M e v S' (h : EvalExpr S E G F M e v S' ) =>
         forall F',
           StringMapProperties.Disjoint F F' ->
           EvalExpr S E G (StringMapProperties.update F F') M e v S' )
-      (* EvalStmt *)
+      (*  EvalStmt *)
       (fun S E G F M stmt S' (h : EvalStmt S E G F M stmt S' ) =>
         forall F',
           StringMapProperties.Disjoint F F' ->
           EvalStmt S E G (StringMapProperties.update F F') M stmt S' )
-      (* EvalExprList *)
+      (*  EvalExprList *)
       (fun Sprev Ecaller G F M ps es vs Snext Ef Sargs l ls
       (h : EvalExprList Sprev Ecaller G F M ps es vs Snext Ef Sargs l ls) =>
         forall F',
@@ -606,6 +653,8 @@ Proof.
 Qed.
 
 
+(*  If a variable expression terminates, then that variable must
+    either be in the local or global environment *)
 Lemma EvalExpr_Var_x_in_E_or_G : forall S E G F M x v S',
   EvalExpr S E G F M (Var x) v S' ->
   StringMap.In x E \/ StringMap.In x G.
@@ -616,6 +665,9 @@ Proof.
 Qed.
 
 
+(*  If an expression e terminates under some context with an initial store S,
+    and some other store S2 is equal to S, then e will also terminate
+    under the original context where S has been replaced with S2 *)
 Lemma S_Equal_EvalExpr : forall S_1 E G F M e v S',
   EvalExpr S_1 E G F M e v S' ->
   forall S_2,
@@ -623,57 +675,60 @@ Lemma S_Equal_EvalExpr : forall S_1 E G F M e v S',
   EvalExpr S_2 E G F M e v S'.
 Proof.
   apply (EvalExpr_mut
-      (* EvalExpr *)
+      (*  EvalExpr *)
       (fun S_1 E G F M e v S' (h : EvalExpr S_1 E G F M e v S' ) =>
         forall S_2,
         NatMap.Equal S_1 S_2 ->
         EvalExpr S_2 E G F M e v S')
-      (* EvalStmt *)
+      (*  EvalStmt *)
       (fun S_1 E G F M stmt S' (h : EvalStmt S_1 E G F M stmt S' ) =>
         forall S_2,
         NatMap.Equal S_1 S_2 ->
         EvalStmt S_2 E G F M stmt S')
-      (* EvalExprList *)
+      (*  EvalExprList *)
       (fun S_1 Ecaller G F M ps es vs Snext Ef Sargs l ls
         (h : EvalExprList S_1 Ecaller G F M ps es vs Snext Ef Sargs l ls) =>
         forall S_2,
         NatMap.Equal S_1 S_2 ->
         EvalExprList S_2 Ecaller G F M ps es vs Snext Ef Sargs l ls)
     ); intros.
-  - (* Num *)
+  - (*  Num *)
     rewrite H in e. constructor; auto.
-  - (* Local var *)
+  - (*  Local var *)
     rewrite H in e. apply E_LocalVar with l; auto. rewrite <- H; auto.
-  - (* Global var *)
+  - (*  Global var *)
      rewrite H in e; apply E_GlobalVar with l; auto. rewrite <- H; auto.
-  - (* ParenExpr *)
+  - (*  ParenExpr *)
      constructor. apply H; auto.
-  - (* UnExpr *)
+  - (*  UnExpr *)
      constructor. apply H; auto.
-  - (* BinExpr *)
+  - (*  BinExpr *)
       apply E_BinExpr with S'.
-      * (* Left operand *)
+      * (*  Left operand *)
         apply H. auto.
-      * (* Right operand *)
+      * (*  Right operand *)
         apply H0; reflexivity.
-  - (* Local assignment *)
+  - (*  Local assignment *)
     rewrite H0 in e1. apply E_Assign_Local with l S'; auto.
-  - (* Global assignment *)
+  - (*  Global assignment *)
     rewrite H0 in e1. apply E_Assign_Global with l S'; auto.
-  - (* Function call *)
+  - (*  Function call *)
     rewrite H2 in e5.
     apply E_FunctionCall with params fstmt fexpr l ls Ef Sargs S' S'' S''' S'''' vs; auto.
-  - (* Macro invocation *)
+  - (*  Macro invocation *)
     apply E_MacroInvocation with params mexpr M' ef; auto.
-  - (* Statements *)
+  - (*  Statements *)
     constructor. rewrite H in e; auto.
-  - (* ExprList (nil) *)
+  - (*  ExprList (nil) *)
     constructor. rewrite H in e; auto.
-  - (* ExprList (cons) *)
+  - (*  ExprList (cons) *)
     apply E_ExprList_cons with Snext; auto.
 Qed.
 
 
+(*  If an expression e terminates under some context with a final store S',
+    and some other store S'2 is equal to S', then e will also terminate
+    under the original context where S' has been replaced with S'2 *)
 Lemma S'_Equal_EvalExpr : forall S E G F M e v S'_1,
   EvalExpr S E G F M e v S'_1 ->
   forall S'_2,
@@ -681,57 +736,61 @@ Lemma S'_Equal_EvalExpr : forall S E G F M e v S'_1,
   EvalExpr S E G F M e v S'_2.
 Proof.
   apply (EvalExpr_mut
-      (* EvalExpr *)
+      (*  EvalExpr *)
       (fun S E G F M e v S'_1 (h : EvalExpr S E G F M e v S'_1 ) =>
         forall S'_2,
         NatMap.Equal S'_1 S'_2 ->
         EvalExpr S E G F M e v S'_2)
-      (* EvalStmt *)
+      (*  EvalStmt *)
       (fun S E G F M stmt S'_1 (h : EvalStmt S E G F M stmt S'_1 ) =>
         forall S'_2,
         NatMap.Equal S'_1 S'_2 ->
         EvalStmt S E G F M stmt S'_2)
-      (* EvalExprList *)
+      (*  EvalExprList *)
       (fun S Ecaller G F M ps es vs Snext_1 Ef Sargs l ls
         (h : EvalExprList S Ecaller G F M ps es vs Snext_1 Ef Sargs l ls) =>
         forall Snext_2,
         NatMap.Equal Snext_1 Snext_2 ->
         EvalExprList S Ecaller G F M ps es vs Snext_2 Ef Sargs l ls)
     ); intros.
-  - (* Num *)
+  - (*  Num *)
     rewrite H in e. constructor; auto.
-  - (* Local var *)
+  - (*  Local var *)
     rewrite H in e. apply E_LocalVar with l; auto.
-  - (* Global var *)
+  - (*  Global var *)
      rewrite H in e; apply E_GlobalVar with l; auto.
-  - (* ParenExpr *)
+  - (*  ParenExpr *)
      constructor. apply H; auto.
-  - (* UnExpr *)
+  - (*  UnExpr *)
      constructor. apply H; auto.
-  - (* BinExpr *)
+  - (*  BinExpr *)
       apply E_BinExpr with S'.
-      * (* Left operand *)
+      * (*  Left operand *)
         apply H. reflexivity.
-      * (* Right operand *)
+      * (*  Right operand *)
         apply H0. auto.
-  - (* Local assignment *)
+  - (*  Local assignment *)
     rewrite H0 in e1. apply E_Assign_Local with l S'; auto.
-  - (* Global assignment *)
+  - (*  Global assignment *)
     rewrite H0 in e1. apply E_Assign_Global with l S'; auto.
-  - (* Function call *)
+  - (*  Function call *)
     rewrite H2 in e5.
     apply E_FunctionCall with params fstmt fexpr l ls Ef Sargs S' S'' S''' S'''' vs; auto.
-  - (* Macro invocation *)
+  - (*  Macro invocation *)
     apply E_MacroInvocation with params mexpr M' ef; auto.
-  - (* Statements *)
+  - (*  Statements *)
     constructor. rewrite H in e; auto.
-  - (* ExprList (nil) *)
+  - (*  ExprList (nil) *)
     constructor. rewrite H in e; auto.
-  - (* ExprList (cons) *)
+  - (*  ExprList (cons) *)
     apply E_ExprList_cons with Snext; auto.
 Qed.
 
 
+(*  If an expression list es terminates under some context with an
+    initial store S, and some other store S2 is equal to S, then es
+    will also terminate under the original context where S has been
+    replaced with S2 *)
 Lemma S_Equal_EvalExprList : forall S_1 Ecaller G F M ps es vs Snext Ef Sargs l ls,
   EvalExprList S_1 Ecaller G F M ps es vs Snext Ef Sargs l ls ->
   forall S_2,
@@ -739,14 +798,17 @@ Lemma S_Equal_EvalExprList : forall S_1 Ecaller G F M ps es vs Snext Ef Sargs l 
   EvalExprList S_2 Ecaller G F M ps es vs Snext Ef Sargs l ls.
 Proof.
   intros S_1 Ecaller G F M ps es vs Snext Ef Sargs l ls H. induction H; intros.
-  - (* ExprList nil *)
+  - (*  ExprList nil *)
     constructor. rewrite H0 in H. auto.
-  - (* ExprList cons *)
+  - (*  ExprList cons *)
     apply E_ExprList_cons with Snext; auto.
     eapply S_Equal_EvalExpr; eauto.
 Qed.
 
 
+(*  If a statement st terminates under some context with an initial store S,
+    and some other store S2 is equal to S, then st will also terminate
+    under the original context where S has been replaced with S2 *)
 Lemma S_Equal_EvalStmt : forall S_1 E G F M st S',
   EvalStmt S_1 E G F M st S' ->
   forall S_2,
@@ -754,11 +816,14 @@ Lemma S_Equal_EvalStmt : forall S_1 E G F M st S',
   EvalStmt S_2 E G F M st S'.
 Proof.
   intros S_1 E G F M st S' H. induction H; intros.
-  - (* Skip *)
+  - (*  Skip *)
     constructor. rewrite H0 in H. auto.
 Qed.
 
 
+(*  If an expression e terminates under some context with a local environment E,
+    and some other local environment E2 is equal to E, then e will also
+    terminate under the original context where E has been replaced with E2 *)
 Lemma E_Equal_EvalExpr : forall S E_1 G F M e v S',
   EvalExpr S E_1 G F M e v S' ->
   forall E_2,
@@ -766,52 +831,55 @@ Lemma E_Equal_EvalExpr : forall S E_1 G F M e v S',
   EvalExpr S E_2 G F M e v S'.
 Proof.
   apply (EvalExpr_mut
-      (* EvalExpr *)
+      (*  EvalExpr *)
       (fun S E_1 G F M e v S' (h : EvalExpr S E_1 G F M e v S' ) =>
         forall E_2,
         StringMap.Equal E_1 E_2 ->
         EvalExpr S E_2 G F M e v S')
-      (* EvalStmt *)
+      (*  EvalStmt *)
       (fun S E_1 G F M stmt S' (h : EvalStmt S E_1 G F M stmt S' ) =>
         forall E_2,
         StringMap.Equal E_1 E_2 ->
         EvalStmt S E_2 G F M stmt S')
-      (* EvalExprList *)
+      (*  EvalExprList *)
       (fun S Ecaller_1 G F M ps es vs Snext Ef Sargs l ls
         (h : EvalExprList S Ecaller_1 G F M ps es vs Snext Ef Sargs l ls) =>
         forall Ecaller_2,
         StringMap.Equal Ecaller_1 Ecaller_2 ->
         EvalExprList S Ecaller_2 G F M ps es vs Snext Ef Sargs l ls)
     ); intros.
-  - (* Num *)
+  - (*  Num *)
     constructor; auto.
-  - (* Local var *)
+  - (*  Local var *)
     apply E_LocalVar with l; auto. rewrite H in m. auto.
-  - (* Global var *)
+  - (*  Global var *)
     apply E_GlobalVar with l; auto. rewrite H in n. auto.
-  - (* ParenExpr *)
+  - (*  ParenExpr *)
     constructor; auto.
-  - (* UnExpr *)
+  - (*  UnExpr *)
     constructor; auto.
-  - (* BinExpr *)
+  - (*  BinExpr *)
     apply E_BinExpr with S'; auto.
-  - (* Local assignment *)
+  - (*  Local assignment *)
     apply E_Assign_Local with l S'; auto. rewrite H0 in m. auto.
-  - (* Global assignment *)
+  - (*  Global assignment *)
     apply E_Assign_Global with l S'; auto. rewrite H0 in n. auto.
-  - (* Function call *)
+  - (*  Function call *)
     apply E_FunctionCall with params fstmt fexpr l ls Ef Sargs S' S'' S''' S'''' vs; auto.
-  - (* Macro invocation *)
+  - (*  Macro invocation *)
     apply E_MacroInvocation with params mexpr M' ef; auto.
-  - (* Statements *)
+  - (*  Statements *)
     constructor; auto.
-  - (* ExprList (nil) *)
+  - (*  ExprList (nil) *)
     constructor; auto.
-  - (* ExprList (cons) *)
+  - (*  ExprList (cons) *)
     apply E_ExprList_cons with Snext; auto.
 Qed.
 
 
+(*  If a statement st terminates under some context with a local environment E,
+    and some other local environment E2 is equal to E, then st will also
+    terminate under the original context where E has been replaced with E2 *)
 Lemma E_Equal_EvalStmt : forall S E_1 G F M st S',
   EvalStmt S E_1 G F M st S' ->
   forall E_2,
@@ -819,11 +887,13 @@ Lemma E_Equal_EvalStmt : forall S E_1 G F M st S',
   EvalStmt S E_2 G F M st S'.
 Proof.
   intros S_1 E G F M st S' H. induction H; intros.
-  - (* Skip *)
+  - (*  Skip *)
     constructor; auto.
 Qed.
 
 
+(*  Given the same context and expression, a program will terminate to the
+    same value and final store every time *)
 Lemma EvalExpr_deterministic : forall S E G F M e v1 S'1,
   EvalExpr S E G F M e v1 S'1 ->
   forall v2 S'2,
@@ -831,80 +901,80 @@ Lemma EvalExpr_deterministic : forall S E G F M e v1 S'1,
   v1 = v2 /\ NatMap.Equal S'1 S'2.
 Proof.
   apply (EvalExpr_mut
-      (* EvalExpr *)
+      (*  EvalExpr *)
       (fun S E G F M e v1 S'1 (h : EvalExpr S E G F M e v1 S'1 ) =>
         forall v2 S'2,
           EvalExpr S E G F M e v2 S'2 ->
           v1 = v2 /\ NatMap.Equal S'1 S'2)
-      (* EvalStmt *)
+      (*  EvalStmt *)
       (fun S E G F M stmt S'1 (h : EvalStmt S E G F M stmt S'1 ) =>
         forall S'2,
           EvalStmt S E G F M stmt S'2 ->
           NatMap.Equal S'1 S'2)
-      (* EvalExprList *)
+      (*  EvalExprList *)
       (fun Sprev Ecaller G F M ps es vs1 Snext1 Ef1 Sargs1 l1 ls1
         (h : EvalExprList Sprev Ecaller G F M ps es vs1 Snext1 Ef1 Sargs1 l1 ls1) =>
         forall vs2 Snext2 Ef2 Sargs2 l2 ls2,
           EvalExprList Sprev Ecaller G F M ps es vs2 Snext2 Ef2 Sargs2 l2 ls2 ->
           vs1 = vs2 /\ NatMap.Equal Snext1 Snext2 /\ StringMap.Equal Ef1 Ef2 /\ NatMap.Equal Sargs1 Sargs2 /\ l1 = l2 /\ ls1 = ls2)
     ); intros; auto.
-  - (* Num *)
+  - (*  Num *)
     inversion_clear H. split; auto.
     rewrite H0 in e. symmetry in e. auto.
-  - (* Local Var *)
+  - (*  Local Var *)
     inversion_clear H.
-    + (* Local *)
+    + (*  Local *)
       assert (l=l0). { eapply StringMapFacts.MapsTo_fun; eauto. }
       subst l0.
       assert (v=v2). { eapply NatMapFacts.MapsTo_fun; eauto. }
       subst v2; split; auto. rewrite <- e. auto.
-    + (* Global (contradiction *)
+    + (*  Global (contradiction *)
       apply StringMap_mapsto_in in m. contradiction.
-  - (* Global Var *)
+  - (*  Global Var *)
     inversion_clear H.
-    + (* Local *)
+    + (*  Local *)
       apply StringMap_mapsto_in in H1. contradiction.
-    + (* Global (contradiction *)
+    + (*  Global (contradiction *)
       assert (l=l0). { eapply StringMapFacts.MapsTo_fun; eauto. }
       subst l0.
       assert (v=v2). { eapply NatMapFacts.MapsTo_fun; eauto. }
       subst v2; split; auto. rewrite <- H0. symmetry. auto.
-  - (* ParenExpr *)
+  - (*  ParenExpr *)
     inversion_clear H0; auto.
-  - (* UnExpr *)
+  - (*  UnExpr *)
       inversion_clear H0.
       destruct H with v0 S'2; auto. subst. auto.
-  - (* BinExpr *)
+  - (*  BinExpr *)
     inversion_clear H1.
-    (* Left operand*)
+    (*  Left operand*)
     assert (v1 = v3 /\ NatMap.Equal S' S'0). { auto. }
     destruct H1; subst.
-    (* Right operand *)
+    (*  Right operand *)
     assert (v2 = v4 /\ NatMap.Equal S'' S'2).
     { apply H0. apply S_Equal_EvalExpr with S'0; auto. symmetry. auto. }
     destruct H1; subst.
     auto.
-  - (* Local Assignment *)
+  - (*  Local Assignment *)
     inversion_clear H0.
-    + (* Local assignment *)
+    + (*  Local assignment *)
       assert (v = v2 /\ NatMap.Equal S' S'0). { auto. }
       destruct H0. subst v2.
       assert (l0 = l). { eapply StringMapFacts.MapsTo_fun; eauto. }
       subst. rewrite <- H3 in e1. auto.
-    + (* Global assignment (contradiction) *)
+    + (*  Global assignment (contradiction) *)
       apply StringMap_mapsto_in in m. contradiction.
-  - (* Global Assignment *)
+  - (*  Global Assignment *)
     inversion_clear H0.
-    + (* Local assignment (contradiction) *)
+    + (*  Local assignment (contradiction) *)
       apply StringMap_mapsto_in in H1. contradiction.
-    + (* Global assignment *)
+    + (*  Global assignment *)
       assert (v = v2 /\ NatMap.Equal S' S'0). { auto. }
       destruct H0. subst v2.
       assert (l0 = l). { eapply StringMapFacts.MapsTo_fun; eauto. }
       subst. auto. rewrite <- H4 in e1. auto.
-  - (* Function call *)
+  - (*  Function call *)
     inversion_clear H2.
-    + (* Function call *)
+    + (*  Function call *)
       assert ((params0, fstmt0, fexpr0) = (params, fstmt, fexpr)).
       { eapply StringMapFacts.MapsTo_fun; eauto. }
       inversion H2; subst params0 fstmt0 fexpr0; clear H2.
@@ -921,13 +991,13 @@ Proof.
         apply E_Equal_EvalExpr with (E_2:=Ef) in H12; auto. }
       destruct H18. subst v2. rewrite H19 in e5.
       rewrite <- e5 in H13. symmetry in H13. auto.
-    + (* Macro invocation (contradiction) *)
+    + (*  Macro invocation (contradiction) *)
       apply StringMap_mapsto_in in H3. contradiction.
-  - (* Macro invocation *)
+  - (*  Macro invocation *)
     inversion_clear H0.
-    + (* Function call (contradiction) *)
+    + (*  Function call (contradiction) *)
       apply StringMap_mapsto_in in m. contradiction.
-    + (* Macro invocation *)
+    + (*  Macro invocation *)
       assert ((params0, mexpr0) = (params, mexpr)).
       { eapply StringMapFacts.MapsTo_fun; eauto. }
       inversion H0. subst params0 mexpr0. clear H0.
@@ -936,12 +1006,12 @@ Proof.
       subst ef0.
       assert (M' = M'0). { rewrite e, H2. reflexivity. }
       subst M'0. apply H; auto. rewrite H0. auto.
-  - (* Statements *)
+  - (*  Statements *)
     inversion_clear H. rewrite e in H0. auto.
-  - (* EvalExprList nil *)
+  - (*  EvalExprList nil *)
     inversion_clear H. rewrite e in H0. repeat (split; auto; try reflexivity).
 
-  - (* EvalExprList cons *)
+  - (*  EvalExprList cons *)
     inversion_clear H1.
     assert (v = v0 /\ NatMap.Equal Snext Snext0). { auto. }
     destruct H1. subst v0.
@@ -953,12 +1023,3 @@ Proof.
     split. rewrite H10. reflexivity.
     auto.
 Qed.
-
-
-
-
-
-
-
-
-
